fairness/pmp_lifting.v
@@ -1,0 +1,112 @@
+From iris.algebra Require Import auth gmap gset excl.
+From iris.proofmode Require Import tactics.
+From trillium.fairness Require Import execution_model.
+From trillium.fairness Require Import fairness fuel resources. 
+From trillium.fairness.lm_rules Require Import resources_updates. 
+
+
+Section PartialModelPredicates.
+  (* Context `{Countable G}.  *)
+  Context `{Countable (locale Λ)}. 
+  Context `{iLM: LiveModel (locale Λ) iM LSI_True}.
+  Context `{EM: ExecutionModel Λ M}.
+  Context `{eGS: em_GS Σ}. 
+  Context `{invGS_gen HasNoLc Σ}.
+  Context {fGS: @fairnessGS _ _ _ _ _ iLM Σ}. 
+  (* Context {PMPP: @PartialModelPredicatesPre (locale Λ) _ _ Σ iM}. *)
+
+  Let update_no_step_enough_fuel_def (extr : execution_trace Λ) 
+      (auxtr : auxiliary_trace M) 
+      (c2 : cfg Λ) (fs : gmap (fmrole iM) nat) (ζ : locale Λ)
+      `(dom fs ≠ ∅)
+      `(locale_step (trace_last extr) (Some ζ) c2): iProp Σ :=
+    has_fuels ζ (S <$> fs) -∗
+    em_msi (trace_last extr) (trace_last auxtr) (em_GS0 := eGS) ==∗
+    ∃ (δ2 : M) (ℓ : mlabel M),
+      ⌜em_valid_state_evolution_fairness (extr :tr[ Some ζ ]: c2)
+      (auxtr :tr[ ℓ ]: δ2)⌝ ∗
+      has_fuels ζ (filter (λ '(k, _), k ∈ dom fs ∖ ∅) fs) ∗
+      em_msi c2 δ2 (em_GS0 := eGS).
+  
+  Let update_fork_split_def (R1 R2: gset (fmrole iM)) tp1 tp2
+       (fs: gmap (fmrole iM) nat)
+        (extr : execution_trace Λ)
+        (auxtr: auxiliary_trace M) ζ efork σ1 σ2
+          `(R1 ## R2)
+          `(fs ≠ ∅)
+          `(R1 ∪ R2 = dom fs)
+         `(trace_last extr = (tp1, σ1))
+          `(locale_step (tp1, σ1) (Some ζ) (tp2, σ2))
+          `((∃ tp1', tp2 = tp1' ++ [efork] ∧ length tp1' = length tp1)): iProp Σ :=
+     has_fuels ζ (S <$> fs) -∗
+     em_msi (trace_last extr) (trace_last auxtr) (em_GS0 := eGS) ==∗
+     ∃ δ2 ℓ, has_fuels (locale_of tp1 efork) (fs ⇂ R2) ∗
+             has_fuels ζ (fs ⇂ R1) ∗
+             (partial_mapping_is {[ locale_of tp1 efork := ∅ ]} -∗
+              em_thread_post (locale_of tp1 efork) (em_GS0 := eGS)) ∗
+             em_msi (tp2, σ2) δ2 (em_GS0 := eGS) ∧ 
+             ⌜em_valid_state_evolution_fairness (extr :tr[Some ζ]: (tp2, σ2)) (auxtr :tr[ℓ]: δ2)⌝.
+ 
+    Let update_step_still_alive_def
+      (extr : execution_trace Λ)
+      (auxtr: auxiliary_trace M)
+       tp1 tp2 σ1 σ2
+       (s1 s2: iM)
+       (fs1 fs2: gmap (fmrole iM) nat)
+      ρ (δ1 : M) ζ fr1 fr_stash
+       (Einvs: coPset)
+     `((live_roles _ s2 ∖ live_roles _ s1) ⊆ fr1 ∪ dom fs1 ∩ dom fs2)
+     `(fr_stash ⊆ dom fs1)
+     `((live_roles _ s1) ∩ (fr_stash ∖ {[ ρ ]}) = ∅)
+     `(dom fs2 ∩ fr_stash = ∅)
+    `(trace_last extr = (tp1, σ1))
+    `(trace_last auxtr = δ1)
+     `(locale_step (tp1, σ1) (Some ζ) (tp2, σ2))
+     `(fmtrans _ s1 (Some ρ) s2)
+      `(valid_new_fuelmap fs1 fs2 s1 s2 ρ (LM := iLM)): iProp Σ :=
+      has_fuels ζ fs1 -∗
+      partial_model_is s1 -∗
+      em_msi (tp1, σ1) δ1 (em_GS0 := eGS) -∗
+      partial_free_roles_are fr1
+      ={ Einvs }=∗
+      ∃ (δ2: M) ℓ,
+      ⌜em_valid_state_evolution_fairness (extr :tr[Some ζ]: (tp2, σ2)) (auxtr :tr[ℓ]: δ2)⌝ ∗
+      has_fuels ζ fs2 ∗
+      partial_model_is s2 ∗
+      em_msi (tp2, σ2) δ2 (em_GS0 := eGS)∗
+      partial_free_roles_are (fr1 ∖ (live_roles _ s2 ∖ (live_roles _ s1 ∪ dom fs1 ∩ dom fs2)) ∪ fr_stash).
+
+    (* TODO: where to place it? *)
+    (* Let partial_free_roles_fuels_disj_def δ fr fs tid: iProp Σ := *)
+    (*     partial_msi δ -∗ partial_free_roles_are fr -∗ has_fuels tid fs -∗ ⌜ fr ## dom fs ⌝. *)
+
+    Let PMP_def (Einvs: coPset): iProp Σ := □ (
+          (∀ extr auxtr c2 fs ζ NE STEP, update_no_step_enough_fuel_def extr auxtr c2 fs ζ NE STEP) ∗
+          (∀ R1 R2 tp1 tp2 fs extr auxtr ζ efork σ1 σ2 DISJ NE DOM LAST STEP POOL, update_fork_split_def R1 R2 tp1 tp2 fs extr auxtr ζ efork σ1 σ2 DISJ NE DOM LAST STEP POOL) ∗
+          (∀ extr auxtr tp1 tp2 σ1 σ2 s1 s2 fs1 fs2 ρ δ1 ζ fr1 fr_stash
+             LR STASH STASH' STASH'' LAST1 LAST2 STEP STEP' VFM,
+              @update_step_still_alive_def extr auxtr tp1 tp2 σ1 σ2 s1 s2 fs1 fs2 ρ δ1 ζ fr1 fr_stash Einvs LR STASH STASH' STASH'' LAST1 LAST2 STEP STEP' VFM)
+).  
+
+    Definition PartialModelPredicates Einvs: iProp Σ := PMP_def Einvs. 
+
+    Lemma Build_PartialModelPredicates Einvs:
+      PMP_def Einvs ⊢ PartialModelPredicates Einvs.
+    Proof. done. Qed. 
+
+    Global Instance PMP_pers: forall Einvs, Persistent (PartialModelPredicates Einvs). 
+    Proof. apply _. Qed.
+
+    Lemma update_no_step_enough_fuel {Einvs} extr auxtr c2 fs ζ NE STEP: 
+      PartialModelPredicates Einvs ⊢ update_no_step_enough_fuel_def extr auxtr c2 fs ζ NE STEP. 
+    Proof. by iIntros "(?&?&?)". Qed.
+    Lemma update_fork_split {Einvs} R1 R2 tp1 tp2 fs extr auxtr ζ efork σ1 σ2 DISJ NE DOM LAST STEP POOL: 
+      PartialModelPredicates Einvs ⊢ update_fork_split_def R1 R2 tp1 tp2 fs extr auxtr ζ efork σ1 σ2 DISJ NE DOM LAST STEP POOL. 
+    Proof. by iIntros "(?&?&?)". Qed.
+    Lemma update_step_still_alive {Einvs} extr auxtr tp1 tp2 σ1 σ2 s1 s2 fs1 fs2 ρ δ1 ζ fr1 fr_stash LR STASH STASH' STASH'' LAST1 LAST2 STEP STEP' VFM:
+      PartialModelPredicates Einvs ⊢ update_step_still_alive_def extr auxtr tp1 tp2 σ1 σ2 s1 s2 fs1 fs2 ρ δ1 ζ fr1 fr_stash Einvs LR STASH STASH' STASH'' LAST1 LAST2 STEP STEP' VFM.
+    Proof. by iIntros "(?&?&?)". Qed. 
+
+    Global Opaque PartialModelPredicates.
+
+End PartialModelPredicates.
